
@prefix attack: <https://ontology.adversaryengagement.org/ae/attack/> .
@prefix identity: <https://ontology.adversaryengagement.org/ae/identity/> .
@prefix objective: <https://ontology.adversaryengagement.org/ae/objective/> .
@prefix owl: <http://www.w3.org/2002/07/owl#> .
@prefix rdfs: <http://www.w3.org/2000/01/rdf-schema#> .
@prefix sh: <http://www.w3.org/ns/shacl#> .
@prefix uco-action: <https://ontology.unifiedcyberontology.org/uco/action/> .
@prefix uco-identity: <https://ontology.unifiedcyberontology.org/uco/identity/> .
@prefix xsd: <http://www.w3.org/2001/XMLSchema#> .




attack:AttackPattern a owl:Class,
        sh:NodeShape ;
    rdfs:label "AttackPattern"@en ;
    rdfs:comment "An attack pattern is a common approach (set of actions) utilized by a person or organization to carry out malicious activity intended to achieve some particular objective (within a particular context) against a targeted victim."@en ;
    rdfs:subClassOf uco-action:ActionPattern ;
    sh:property
      [
        sh:class engagement:Objective ;
	sh:nodeKind sh:IRI ;
	sh:path objective:hasObjective
      ] ;
    sh:targetClass attack:AttackPattern .



attack:CyberKillChain a owl:Class,
        sh:NodeShape ;
    rdfs:label "CyberKillChain"@en ;
    rdfs:comment "An cyber kill chain is an ordered sequence of actions or events describing a lifecycle from some framework."@en ;
    rdfs:subClassOf uco-action:ActionLifecycle ;
    sh:targetClass attack:CyberKillChain .




attack:DefensePattern a owl:Class,
        sh:NodeShape ;
    rdfs:label "AttackPattern"@en ;
    rdfs:comment "A defense pattern is a common approach (set of actions) utilized by a person or organization to carry out defensive activity intended to achieve some particular objective (within a particular context) against malicious activity."@en ;
    rdfs:subClassOf uco-action:ActionPattern ;
    sh:property
      [
        sh:class engagement:Objective ;
	sh:nodeKind sh:IRI ;
	sh:path objective:hasObjective 
      ] ;
    sh:targetClass attack:DefensePattern .